Classes/Numerical.v
@@ -1,0 +1,11 @@
+Require Import Language.Statements.
+Require Import Types.State.
+
+Class Numerical {T  : Type} {state : (Type -> Type)} (N : Type) 
+  : Type :=
+{
+  ensure_numerical : T -> state N;
+  plus_op : N -> N -> N;
+  mult_op : N -> N -> N;
+}.
+
