Instances/Numerical/Nat.v
@@ -1,0 +1,19 @@
+Require Import Classes.Numerical.
+Require Import Types.AbstractStore.
+Require Import Language.Statements.
+Require Import Types.State.
+Require Import Types.Result.
+
+Definition ensure_nat (v : cvalue) : State nat :=
+  fun st => match v with
+            | VNat x => returnR nat store x st
+            | _ => crashed _ _
+            end.
+
+Global Instance nat_numerical : Numerical nat :=
+{
+  ensure_numerical := ensure_nat;
+  plus_op := plus;
+  mult_op := mult;
+}.
+
