Instances/Numerical/Parity.v
@@ -1,0 +1,20 @@
+Require Import Classes.Numerical.
+Require Import Types.Parity.
+Require Import Language.Statements.
+Require Import Types.State.
+Require Import Types.Result.
+Require Import Types.AbstractStore.
+
+Definition ensure_par (v : avalue) : AbstractState parity :=
+  fun st => match v with
+            | VParity x => returnRA parity abstract_store x st
+            | _ => crashedA _ _
+            end.
+
+Global Instance parity_numerical : Numerical parity :=
+{
+  ensure_numerical := ensure_par;
+  plus_op := parity_plus;
+  mult_op := parity_mult;
+}.
+
